theory CustomizedFull
  imports Main
begin

(* 修正1: 提供非空性证明 *)
typedef Even = "{x::nat. x mod 2 = 0}"
proof
  show "0 \<in> {x::nat. x mod 2 = 0}" by simp
qed

term Rep_Even
(* 输出 "Rep_Even" :: "Even \<Rightarrow> nat" *)
term Abs_Even
(* 输出 "Abs_Even" :: "nat \<Rightarrow> Even" *)

(* 修正2: 正确的类型类实例化语法 *)
instantiation Even :: zero
begin
definition zero_Even_def: "0 = Abs_Even 0"
instance by standard
end

term "0::Even"
(* 输出 "0" :: "Even" *)

instantiation Even :: one
begin  
definition one_Even_def: "1 = Abs_Even 2"
instance by standard
end

term "1::Even"
(* 输出 "1" :: "Even" *)

definition SUC :: "Even \<Rightarrow> Even"
  where "SUC n \<equiv> Abs_Even (Suc (Suc (Rep_Even n)))"

definition ADD :: "Even \<Rightarrow> Even \<Rightarrow> Even"
  where "ADD m n \<equiv> Abs_Even ((Rep_Even m) + (Rep_Even n))"

(* 修正3: 为引理提供证明 *)
lemma suc_zero_eq_one: "SUC 0 = 1"
proof -
  have "SUC 0 = Abs_Even (Suc (Suc (Rep_Even 0)))" 
    by (simp add: SUC_def)
  also have "... = Abs_Even (Suc (Suc 0))"
    by (simp add: zero_Even_def Rep_Even_inverse)
  also have "... = Abs_Even 2"
    by simp
  also have "... = 1"
    by (simp add: one_Even_def)
  finally show ?thesis .
qed

lemma add_suc_suc: "ADD (SUC 0) (SUC 0) = SUC (SUC 0)"  
proof -
  have "ADD (SUC 0) (SUC 0) = Abs_Even (Rep_Even (SUC 0) + Rep_Even (SUC 0))"
    by (simp add: ADD_def)
  also have "SUC 0 = Abs_Even 2"
    by (simp add: SUC_def zero_Even_def Rep_Even_inverse)
  also have "Rep_Even (Abs_Even 2) = 2"
    by (simp add: Abs_Even_inverse)
  also have "Abs_Even (2 + 2) = Abs_Even 4"
    by simp
  also have "SUC (SUC 0) = Abs_Even (Suc (Suc (Rep_Even (SUC 0))))"
    by (simp add: SUC_def)
  also have "... = Abs_Even (Suc (Suc 2))"
    by (simp add: SUC_def zero_Even_def Rep_Even_inverse Abs_Even_inverse)
  also have "... = Abs_Even 4"
    by simp
  finally show ?thesis by simp
qed

end